AP/AP/FreshA/Nbhd.lean
@@ -6,6 +6,71 @@ namespace AP
 
 theorem AState.aHwsDisj_nbhd_pw {s : State} {fsp : FSP} [hs : AState s]
 (h : s.aHwsDisj fsp) : s.aHwsDisj # fsp.insertSet 3 # s.aPos.nbhd s.pw |>.toSet := by
+  generalize hb : Set'.ofList (s.aPos.nbhd s.pw) = set
   replace h := exi_fresh1_of_aHwsDisj h
   choose a ha using h
+  
+  have h : (s.aPos.nbhd s.pw).toSet = set.toSet
+  · simp [←hb]
+  rw [h]; clear h
+  
+  have h₁ := State.aPtsSimNcard_spec_of_fresh1 ha set
+  
+  generalize hf : (λ d => s.aPtsSimNcard ⟨a, d⟩ set.toSet) = f
+  replace h₁ : ∀ (d : DStrat) [d.WF], ∃ n, f d = some n ∧ n ≤ set.size; grind
+  
+  generalize hg : (λ d => f d |>.iget) = g
+  have h₂ : ∀ (d : DStrat) [d.WF], g d ≤ set.size; grind
+  
+  have h₃ : ∃ (d : DStrat), d.WF ∧ ∀ (d₁ : DStrat) [d₁.WF], g d₁ ≤ g d
+  ·
+    generalize set.size = N at h₂
+    induction N
+    ·
+      simp at h₂
+      use default, inferInstance
+      intro d₁ hd₁
+      simp [h₂]
+    nm N ih
+    by_cases h₃ : ∃ (d : DStrat), d.WF ∧ g d = N + 1
+    ·
+      choose d hd h₃ using h₃
+      use d, hd
+      intro d₁ hd₁
+      grind
+    apply ih; grind
+  
+  choose d hd h₃ using h₃
+  clear h₂
+  
+  replace h₁ : ∀ (d : DStrat) [d.WF], ∃ n, n ≠ 0 ∧ f d = some n ∧ n ≤ g d
+  ·
+    intro d₁ hd₁
+    specialize h₁ d₁
+    choose n h₁ h₄ using h₁
+    use n; simp [h₁]
+    symm; split_ands; grind
+    rintro rfl
+    simp [←hf] at h₁
+    have h₅ := State.aWins_of_aWinsDisj (ha.2.1 d₁ hd₁) 1
+    simp at h₅
+    choose s₁ h₅ using h₅
+    specialize h₁ 0 s s₁
+    simp at h₁
+    specialize h₁ h₅
+    apply h₁; clear h₁
+    simp [←hb]
+    rw [Point.dist_comm]
+    rw [AState.tr_eq_some_iff] at h₅
+    grind
+  
+  have h₄ : ∃ n s₁, AState s₁ ∧ sys.simulate (Strat.f ⟨a, d⟩) s n = (s₁, 0) ∧
+    s₁.aPos ∈ set ∧ ∀ k s₂, sys.simulate (Strat.f ⟨a, d⟩) s₁ k = (s₂, 0) → s₁.aPos ∉ set
+  ·
+    specialize h₁ d
+    choose N h₁ h₄ h₅ using h₁
+    clear h₅
+    simp [←hf] at h₄
+    sorry
+  
   sorry
